<?xml version="1.0" encoding="UTF-8"?>
<rdf:RDF xmlns:adms="http://www.w3.org/ns/adms#"
         xmlns:at-voc="http://publications.europa.eu/resource/authority/"
         xmlns:bibo="http://purl.org/ontology/bibo/"
         xmlns:cc="http://creativecommons.org/ns#"
         xmlns:cccev="http://data.europa.eu/m8g/"
         xmlns:clv="http://data.europa.eu/m8g/"
         xmlns:cpov="http://data.europa.eu/m8g/"
         xmlns:cpsv="http://data.europa.eu/m8g/"
         xmlns:cpv="http://data.europa.eu/m8g/"
         xmlns:cv="http://data.europa.eu/m8g/"
         xmlns:dc="http://purl.org/dc/elements/1.1/"
         xmlns:dct="http://purl.org/dc/terms/"
         xmlns:foaf="http://xmlns.com/foaf/0.1/"
         xmlns:geosparql="http://www.opengis.net/ont/geosparql#"
         xmlns:locn="http://www.w3.org/ns/locn#"
         xmlns:org="http://www.w3.org/ns/org#"
         xmlns:owl="http://www.w3.org/2002/07/owl#"
         xmlns:person="http://www.w3.org/ns/person#"
         xmlns:prov="https://www.w3.org/ns/prov#"
         xmlns:rdf="http://www.w3.org/1999/02/22-rdf-syntax-ns#"
         xmlns:rdfs="http://www.w3.org/2000/01/rdf-schema#"
         xmlns:skos="http://www.w3.org/2004/02/skos/core#"
         xmlns:time="http://www.w3.org/2006/time#"
         xmlns:vann="http://purl.org/vocab/vann/"
         xmlns:xhtml="https://www.w3.org/1999/xhtml/vocab#"
         xmlns:xsd="http://www.w3.org/2001/XMLSchema#">
   <owl:Ontology rdf:about="http://data.europa.eu/a4g/ontology#core">
      <owl:imports rdf:resource="http://xmlns.com/foaf/0.1/"/>
      <owl:imports rdf:resource="http://purl.org/dc/terms/"/>
      <owl:imports rdf:resource="http://www.w3.org/ns/org#"/>
      <owl:imports rdf:resource="http://www.w3.org/2004/02/skos/core"/>
      <owl:imports rdf:resource="http://publications.europa.eu/resource/authority/"/>
      <owl:imports rdf:resource="http://www.w3.org/2006/time"/>
      <owl:imports rdf:resource="http://www.w3.org/ns/locn"/>
      <owl:imports rdf:resource="https://data.europa.eu/m8g/"/>
      <owl:imports rdf:resource="http://data.europa.eu/m8g/"/>
      <owl:imports rdf:resource="http://data.europa.eu/m8g/"/>
      <owl:imports rdf:resource="http://data.europa.eu/m8g/"/>
      <owl:imports rdf:resource="http://data.europa.eu/m8g/"/>
      <owl:imports rdf:resource="https://data.europa.eu/m8g/"/>
      <owl:imports rdf:resource="http://www.opengis.net/ont/geosparql"/>
      <owl:imports rdf:resource="http://www.w3.org/ns/person"/>
      <owl:imports rdf:resource="http://www.w3.org/ns/adms"/>
      <owl:imports rdf:resource="https://www.w3.org/ns/prov"/>
      <owl:imports rdf:resource="https://www.w3.org/1999/xhtml/vocab"/>
      <dct:title xml:lang="en">ePO Core core</dct:title>
      <dct:description xml:lang="en">This artefact provides the definitions for the eProcurement Ontology Core.         This artefact excludes the restrictions.         The eProcurement Ontology describes objects and concepts, with definitions, attributes and relationships which are present within the European public procurement domain.         The provision of these concepts provides the basis for a common understanding of the domain for all stakeholders ensuring the quality of data exchange and transparency.</dct:description>
      <dct:publisher>http://publications.europa.eu/resource/authority/corporate-body/PUBL</dct:publisher>
      <rdfs:comment>This version is automatically generated from core_public_organisation_CM.xml on 2023-10-11</rdfs:comment>
      <rdfs:seeAlso rdf:resource="https://github.com/eprocurementontology/eprocurementontology"/>
      <rdfs:seeAlso rdf:resource="https://joinup.ec.europa.eu/collection/eprocurement/solution/eprocurement-ontology/about"/>
      <rdfs:seeAlso rdf:resource="https://op.europa.eu/en/web/eu-vocabularies/e-procurement"/>
      <rdfs:seeAlso rdf:resource="https://docs.ted.europa.eu/EPO/latest/index.html"/>
      <dct:issued rdf:datatype="http://www.w3.org/2001/XMLSchema#date">2023-10-11</dct:issued>
      <owl:versionInfo>3.1.0</owl:versionInfo>
      <owl:incompatibleWith>2.1.0</owl:incompatibleWith>
      <owl:versionIRI rdf:resource="http://data.europa.eu/a4g/ontology#core-3.1.0"/>
      <bibo:status>Semantic Specification Realease</bibo:status>
      <owl:priorVersion>3.0.1</owl:priorVersion>
      <vann:preferredNamespaceUri>http://data.europa.eu/a4g/ontology#</vann:preferredNamespaceUri>
      <vann:preferredNamespacePrefix>epo</vann:preferredNamespacePrefix>
      <dct:rights>The Commission’s reuse policy is implemented by Commission Decision2011/833/EU of 12 December 2011 on the reuse of Commission documents          (OJ L 330,14.12.2011, p. 39 – https://eur-lex.europa.eu/eli/dec/2011/833/oj). Unlessotherwise noted, the reuse of this document is authorised under the          CreativeCommons Attribution 4.0 International (CC BY 4.0) licence (https://creativecommons.org/licenses/by/4.0/).This means that reuse is allowed, provided          that appropriate credit is given and any changes are indicated.</dct:rights>
      <dct:license rdf:resource="http://creativecommons.org/licenses/by-sa/4.0"/>
      <cc:attributionName>European Union</cc:attributionName>
      <cc:attributionURL rdf:resource="http://publications.europa.eu/resource/authority/corporate-body/EURUN"/>
   </owl:Ontology>
   <owl:Class rdf:about="http://data.europa.eu/m8g/ReferenceFramework"/>
   <rdf:Description rdf:about="http://data.europa.eu/m8g/ReferenceFramework">
      <skos:prefLabel xml:lang="en">Reference framework</skos:prefLabel>
   </rdf:Description>
   <rdf:Description rdf:about="http://data.europa.eu/m8g/ReferenceFramework">
      <skos:definition xml:lang="en">Legislation or official policy from which Requirements are derived.</skos:definition>
   </rdf:Description>
   <owl:Class rdf:about="http://data.europa.eu/m8g/ImageObject"/>
   <rdf:Description rdf:about="http://data.europa.eu/m8g/ImageObject">
      <skos:prefLabel xml:lang="en">Image object</skos:prefLabel>
   </rdf:Description>
   <rdf:Description rdf:about="http://data.europa.eu/m8g/ImageObject">
      <skos:definition xml:lang="en">A logo to describe / represent the PublicOrganization.</skos:definition>
   </rdf:Description>
   <owl:Class rdf:about="http://data.europa.eu/m8g/PublicOrganisation"/>
   <rdf:Description rdf:about="http://data.europa.eu/m8g/PublicOrganisation">
      <skos:prefLabel xml:lang="en">Public organisation</skos:prefLabel>
   </rdf:Description>
   <rdf:Description rdf:about="http://data.europa.eu/m8g/PublicOrganisation">
      <skos:definition xml:lang="en">An Organization that is defined as being part of the public sector by a legal framework at any level.</skos:definition>
   </rdf:Description>
   <owl:Class rdf:about="http://xmlns.com/foaf/0.1/Document"/>
   <rdf:Description rdf:about="http://xmlns.com/foaf/0.1/Document">
      <skos:prefLabel xml:lang="en">Document</skos:prefLabel>
   </rdf:Description>
   <rdf:Description rdf:about="http://xmlns.com/foaf/0.1/Document">
      <skos:definition xml:lang="en">A self-contained collection of information in a readable format.</skos:definition>
   </rdf:Description>
   <owl:Class rdf:about="http://www.w3.org/ns/org#ChangeEvent"/>
   <rdf:Description rdf:about="http://www.w3.org/ns/org#ChangeEvent">
      <skos:prefLabel xml:lang="en">Change event</skos:prefLabel>
   </rdf:Description>
   <rdf:Description rdf:about="http://www.w3.org/ns/org#ChangeEvent">
      <skos:definition xml:lang="en">An event which resulted in a major change to an Organization such as a merger or complete restructuring.</skos:definition>
   </rdf:Description>
   <owl:Class rdf:about="http://www.w3.org/ns/org#Organization"/>
   <rdf:Description rdf:about="http://www.w3.org/ns/org#Organization">
      <skos:prefLabel xml:lang="en">Organization</skos:prefLabel>
   </rdf:Description>
   <rdf:Description rdf:about="http://www.w3.org/ns/org#Organization">
      <skos:definition xml:lang="en">A collection of people organized together into a community or other social, commercial or political structure. The group has some common purpose or reason for existence which goes beyond the set of people belonging to it and can act as an Agent. Organizations are often decomposable into hierarchical structures.</skos:definition>
   </rdf:Description>
   <owl:Class rdf:about="http://www.w3.org/ns/org#OrganizationalUnit"/>
   <rdf:Description rdf:about="http://www.w3.org/ns/org#OrganizationalUnit">
      <skos:prefLabel xml:lang="en">Organizational unit</skos:prefLabel>
   </rdf:Description>
   <rdf:Description rdf:about="http://www.w3.org/ns/org#OrganizationalUnit">
      <skos:definition xml:lang="en">A subdivision of Organization which is part of this Organization.</skos:definition>
   </rdf:Description>
   <owl:Class rdf:about="http://www.w3.org/2006/time#TemporalEntity"/>
   <rdf:Description rdf:about="http://www.w3.org/2006/time#TemporalEntity">
      <skos:prefLabel xml:lang="en">Temporal entity</skos:prefLabel>
   </rdf:Description>
   <rdf:Description rdf:about="http://www.w3.org/2006/time#TemporalEntity">
      <skos:definition xml:lang="en">A temporal interval or instant.</skos:definition>
   </rdf:Description>
   <owl:Class rdf:about="http://data.europa.eu/m8g/PublicOrganisation">
      <rdfs:subClassOf rdf:resource="http://www.w3.org/ns/org#Organization"/>
   </owl:Class>
   <owl:Class rdf:about="http://www.w3.org/ns/org#OrganizationalUnit">
      <rdfs:subClassOf rdf:resource="http://www.w3.org/ns/org#Organization"/>
   </owl:Class>
   <owl:Class rdf:about="http://data.europa.eu/m8g/PublicOrganisation">
      <rdfs:subClassOf rdf:resource="http://www.w3.org/ns/org#Organization"/>
   </owl:Class>
   <owl:Class rdf:about="http://www.w3.org/ns/org#OrganizationalUnit">
      <rdfs:subClassOf rdf:resource="http://www.w3.org/ns/org#Organization"/>
   </owl:Class>
   <rdf:Description rdf:about="http://publications.europa.eu/resource/authority/atu-type">
      <skos:editorialNote xml:lang="en">the URI in core voc is wrong; a dataset URI instead the conceptScheme URI.</skos:editorialNote>
   </rdf:Description>
   <owl:ObjectProperty rdf:about="http://data.europa.eu/m8g/implements"/>
   <rdf:Description rdf:about="http://data.europa.eu/m8g/implements">
      <skos:prefLabel xml:lang="en">Implements</skos:prefLabel>
   </rdf:Description>
   <owl:ObjectProperty rdf:about="http://data.europa.eu/m8g/hasFormalFramework"/>
   <rdf:Description rdf:about="http://data.europa.eu/m8g/hasFormalFramework">
      <skos:prefLabel xml:lang="en">Has formal framework</skos:prefLabel>
   </rdf:Description>
   <owl:ObjectProperty rdf:about="http://data.europa.eu/m8g/logo"/>
   <rdf:Description rdf:about="http://data.europa.eu/m8g/logo">
      <skos:prefLabel xml:lang="en">Logo</skos:prefLabel>
   </rdf:Description>
   <owl:ObjectProperty rdf:about="http://www.w3.org/ns/org#memberOf"/>
   <rdf:Description rdf:about="http://www.w3.org/ns/org#memberOf">
      <skos:prefLabel xml:lang="en">Member of</skos:prefLabel>
   </rdf:Description>
   <owl:ObjectProperty rdf:about="http://www.w3.org/ns/org#hasMember"/>
   <rdf:Description rdf:about="http://www.w3.org/ns/org#hasMember">
      <skos:prefLabel xml:lang="en">Has member</skos:prefLabel>
   </rdf:Description>
   <owl:ObjectProperty rdf:about="http://data.europa.eu/m8g/contactPoint"/>
   <rdf:Description rdf:about="http://data.europa.eu/m8g/contactPoint">
      <skos:prefLabel xml:lang="en">Contact point</skos:prefLabel>
   </rdf:Description>
   <rdf:Description rdf:about="http://data.europa.eu/m8g/contactPoint">
      <skos:definition xml:lang="en">The main contact information of the resource. (cpov:PublicOrganisation -&gt; cv:ContactPoint (+cpv:contactPoint)) </skos:definition>
   </rdf:Description>
   <owl:ObjectProperty rdf:about="http://www.w3.org/ns/org#purpose"/>
   <rdf:Description rdf:about="http://www.w3.org/ns/org#purpose">
      <skos:prefLabel xml:lang="en">Purpose</skos:prefLabel>
   </rdf:Description>
   <rdf:Description rdf:about="http://www.w3.org/ns/org#purpose">
      <skos:definition xml:lang="en">This property describes the reasons of existence of an Organization. (cpov:PublicOrganisation -&gt; org:purpose (+org:purpose)) </skos:definition>
   </rdf:Description>
   <owl:ObjectProperty rdf:about="https://www.w3.org/1999/xhtml/vocab#prev"/>
   <rdf:Description rdf:about="https://www.w3.org/1999/xhtml/vocab#prev">
      <skos:prefLabel xml:lang="en">Prev</skos:prefLabel>
   </rdf:Description>
   <owl:ObjectProperty rdf:about="https://www.w3.org/1999/xhtml/vocab#next"/>
   <rdf:Description rdf:about="https://www.w3.org/1999/xhtml/vocab#next">
      <skos:prefLabel xml:lang="en">Next</skos:prefLabel>
   </rdf:Description>
   <owl:ObjectProperty rdf:about="http://www.w3.org/ns/locn#address"/>
   <rdf:Description rdf:about="http://www.w3.org/ns/locn#address">
      <skos:prefLabel xml:lang="en">Address</skos:prefLabel>
   </rdf:Description>
   <rdf:Description rdf:about="http://www.w3.org/ns/locn#address">
      <skos:definition xml:lang="en">The Address of a Public Organization. (cpov:PublicOrganisation -&gt; locn:Address (+locn:address)) </skos:definition>
   </rdf:Description>
   <owl:ObjectProperty rdf:about="http://www.w3.org/ns/org#classification"/>
   <rdf:Description rdf:about="http://www.w3.org/ns/org#classification">
      <skos:prefLabel xml:lang="en">Classification</skos:prefLabel>
   </rdf:Description>
   <rdf:Description rdf:about="http://www.w3.org/ns/org#classification">
      <skos:definition xml:lang="en">The categorisation of the Public Organization. (cpov:PublicOrganisation -&gt; org:classification (+org:classification)) </skos:definition>
   </rdf:Description>
   <owl:ObjectProperty rdf:about="http://purl.org/dc/terms/spatial"/>
   <rdf:Description rdf:about="http://purl.org/dc/terms/spatial">
      <skos:prefLabel xml:lang="en">Spatial</skos:prefLabel>
   </rdf:Description>
   <rdf:Description rdf:about="http://purl.org/dc/terms/spatial">
      <skos:definition xml:lang="en">This property links an Organization to the Administrative Region(s) that it covers. (cpov:PublicOrganisation -&gt; at-voc:atu-type (+dct:spatial)) </skos:definition>
   </rdf:Description>
   <owl:ObjectProperty rdf:about="http://www.w3.org/ns/org#originalOrganization"/>
   <rdf:Description rdf:about="http://www.w3.org/ns/org#originalOrganization">
      <skos:prefLabel xml:lang="en">Original organization</skos:prefLabel>
   </rdf:Description>
   <owl:ObjectProperty rdf:about="http://www.w3.org/ns/org#changedBy"/>
   <rdf:Description rdf:about="http://www.w3.org/ns/org#changedBy">
      <skos:prefLabel xml:lang="en">Changed by</skos:prefLabel>
   </rdf:Description>
   <owl:ObjectProperty rdf:about="http://www.w3.org/ns/org#resultingOrganization"/>
   <rdf:Description rdf:about="http://www.w3.org/ns/org#resultingOrganization">
      <skos:prefLabel xml:lang="en">Resulting organization</skos:prefLabel>
   </rdf:Description>
   <owl:ObjectProperty rdf:about="http://www.w3.org/ns/org#resultedFrom"/>
   <rdf:Description rdf:about="http://www.w3.org/ns/org#resultedFrom">
      <skos:prefLabel xml:lang="en">Resulted from</skos:prefLabel>
   </rdf:Description>
   <owl:ObjectProperty rdf:about="http://www.w3.org/ns/adms#identifier"/>
   <rdf:Description rdf:about="http://www.w3.org/ns/adms#identifier">
      <skos:prefLabel xml:lang="en">Identifier</skos:prefLabel>
   </rdf:Description>
   <owl:ObjectProperty rdf:about="http://xmlns.com/foaf/0.1/homepage"/>
   <rdf:Description rdf:about="http://xmlns.com/foaf/0.1/homepage">
      <skos:prefLabel xml:lang="en">Homepage</skos:prefLabel>
   </rdf:Description>
   <rdf:Description rdf:about="http://xmlns.com/foaf/0.1/homepage">
      <skos:definition xml:lang="en">The official home page of the Public Organization. (cpov:PublicOrganisation -&gt; foaf:Document (+foaf:homepage)) </skos:definition>
   </rdf:Description>
   <owl:ObjectProperty rdf:about="http://www.w3.org/ns/org#unitOf"/>
   <rdf:Description rdf:about="http://www.w3.org/ns/org#unitOf">
      <skos:prefLabel xml:lang="en">Unit of</skos:prefLabel>
   </rdf:Description>
   <owl:ObjectProperty rdf:about="http://www.w3.org/ns/org#hasUnit"/>
   <rdf:Description rdf:about="http://www.w3.org/ns/org#hasUnit">
      <skos:prefLabel xml:lang="en">Has unit</skos:prefLabel>
   </rdf:Description>
   <owl:ObjectProperty rdf:about="http://www.w3.org/ns/org#hasSubOrganization"/>
   <rdf:Description rdf:about="http://www.w3.org/ns/org#hasSubOrganization">
      <skos:prefLabel xml:lang="en">Has sub organization</skos:prefLabel>
   </rdf:Description>
   <owl:ObjectProperty rdf:about="http://www.w3.org/ns/org#subOrganizationOf"/>
   <rdf:Description rdf:about="http://www.w3.org/ns/org#subOrganizationOf">
      <skos:prefLabel xml:lang="en">Sub organization of</skos:prefLabel>
   </rdf:Description>
   <owl:ObjectProperty rdf:about="http://data.europa.eu/m8g/frequency"/>
   <rdf:Description rdf:about="http://data.europa.eu/m8g/frequency">
      <skos:prefLabel xml:lang="en">Frequency</skos:prefLabel>
   </rdf:Description>
   <rdf:Description rdf:about="http://data.europa.eu/m8g/frequency">
      <skos:definition xml:lang="en">The recurrence of an instant or period.
 (time:TemporalEntity -&gt; cpov:frequency (+cpov:frequency)) </skos:definition>
   </rdf:Description>
   <owl:ObjectProperty rdf:about="http://data.europa.eu/m8g/specialOpeningHoursSpecification"/>
   <rdf:Description rdf:about="http://data.europa.eu/m8g/specialOpeningHoursSpecification">
      <skos:prefLabel xml:lang="en">Special opening hours specification</skos:prefLabel>
   </rdf:Description>
   <rdf:Description rdf:about="http://data.europa.eu/m8g/specialOpeningHoursSpecification">
      <skos:definition xml:lang="en">The time during which the Contact Point is not available. (cv:ContactPoint -&gt; time:TemporalEntity (+cpov:specialOpeningHoursSpecification)) </skos:definition>
   </rdf:Description>
   <owl:ObjectProperty rdf:about="http://data.europa.eu/m8g/openingHours"/>
   <rdf:Description rdf:about="http://data.europa.eu/m8g/openingHours">
      <skos:prefLabel xml:lang="en">Opening hours</skos:prefLabel>
   </rdf:Description>
   <rdf:Description rdf:about="http://data.europa.eu/m8g/openingHours">
      <skos:definition xml:lang="en">The time at which the Contact Point is normally available. (cv:ContactPoint -&gt; time:TemporalEntity (+cpov:openingHours)) </skos:definition>
   </rdf:Description>
   <owl:DatatypeProperty rdf:about="http://purl.org/dc/terms/identifier"/>
   <rdf:Description rdf:about="http://purl.org/dc/terms/identifier">
      <skos:prefLabel xml:lang="en">Identifier</skos:prefLabel>
   </rdf:Description>
   <rdf:Description rdf:about="http://purl.org/dc/terms/identifier">
      <skos:definition xml:lang="en">An unambiguous reference to a Reference Framework. (cccev:ReferenceFramework) </skos:definition>
   </rdf:Description>
   <owl:DatatypeProperty rdf:about="http://www.w3.org/2004/02/skos/core#altLabel"/>
   <rdf:Description rdf:about="http://www.w3.org/2004/02/skos/core#altLabel">
      <skos:prefLabel xml:lang="en">Alt label</skos:prefLabel>
   </rdf:Description>
   <rdf:Description rdf:about="http://www.w3.org/2004/02/skos/core#altLabel">
      <skos:definition xml:lang="en">An alternative or informal name(s) of a Public Organization, irrespective of language. (cpov:PublicOrganisation) </skos:definition>
   </rdf:Description>
   <owl:DatatypeProperty rdf:about="http://purl.org/dc/terms/description"/>
   <rdf:Description rdf:about="http://purl.org/dc/terms/description">
      <skos:prefLabel xml:lang="en">Description</skos:prefLabel>
   </rdf:Description>
   <rdf:Description rdf:about="http://purl.org/dc/terms/description">
      <skos:definition xml:lang="en">The textual description of the Public Organization. (cpov:PublicOrganisation) A textual explanation of the event. (org:ChangeEvent) A textual representation of the Temporal Entity. (time:TemporalEntity) </skos:definition>
   </rdf:Description>
   <owl:DatatypeProperty rdf:about="http://www.w3.org/2004/02/skos/core#prefLabel"/>
   <rdf:Description rdf:about="http://www.w3.org/2004/02/skos/core#prefLabel">
      <skos:prefLabel xml:lang="en">Pref label</skos:prefLabel>
   </rdf:Description>
   <rdf:Description rdf:about="http://www.w3.org/2004/02/skos/core#prefLabel">
      <skos:definition xml:lang="en">A preferred label is used to provide the primary, legally recognised name of the Public Organization, as defined in the ORG Ontology. (cpov:PublicOrganisation) </skos:definition>
   </rdf:Description>
   <owl:DatatypeProperty rdf:about="https://www.w3.org/ns/prov#endedAtTime"/>
   <rdf:Description rdf:about="https://www.w3.org/ns/prov#endedAtTime">
      <skos:prefLabel xml:lang="en">Ended at time</skos:prefLabel>
   </rdf:Description>
   <rdf:Description rdf:about="https://www.w3.org/ns/prov#endedAtTime">
      <skos:definition xml:lang="en">The time instant when the state of the organisation update was terminated (org:ChangeEvent) </skos:definition>
   </rdf:Description>
   <owl:DatatypeProperty rdf:about="https://www.w3.org/ns/prov#startedAtTime"/>
   <rdf:Description rdf:about="https://www.w3.org/ns/prov#startedAtTime">
      <skos:prefLabel xml:lang="en">Started at time</skos:prefLabel>
   </rdf:Description>
   <rdf:Description rdf:about="https://www.w3.org/ns/prov#startedAtTime">
      <skos:definition xml:lang="en">The time instant when the state of the organisation update was initiated. (org:ChangeEvent) </skos:definition>
   </rdf:Description>
</rdf:RDF>
